@prefix dct: <http://purl.org/dc/terms/> .
@prefix evtAgRole: <http://id.loc.gov/vocabulary/preservation/eventRelatedAgentRole/> .
@prefix evtObjRole: <http://id.loc.gov/vocabulary/preservation/eventRelatedObjectRole/> .
@prefix evtOutcome: <http://id.loc.gov/vocabulary/preservation/eventOutcome/> .
@prefix evtType: <http://id.loc.gov/vocabulary/preservation/eventType> .
@prefix foaf: <http://xmlns.com/foaf/0.1/> .
@prefix haEvt: <http://data.hetarchief.be/ns/event/> .
@prefix premis: <http://www.loc.gov/premis/rdf/v3/> .
@prefix prov: <http://www.w3.org/ns/prov#> .
@prefix rdf: <http://www.w3.org/1999/02/22-rdf-syntax-ns#> .
@prefix rdfs: <http://www.w3.org/2000/01/rdf-schema#> .
@prefix skos: <http://www.w3.org/2004/02/skos/core#> .
@prefix vann: <http://purl.org/vocab/vann/> .
@prefix xsd: <http://www.w3.org/2001/XMLSchema#> .
@prefix owl: <http://www.w3.org/2002/07/owl#> .
@prefix schema: <https://schema.org/> .
@prefix pav: <http://purl.org/pav/> .


<https://data.hetarchief.be/ns/event>  a owl:Ontology;
    vann:preferredNamespacePrefix "haEvt" ;
    vann:preferredNamespaceUri "http://data.hetarchief.be/ns/events/" ;
    dct:author  [
        schema:name   "Milan Valadou" ;
        schema:email  "milan.valadou@meemoo.be"
    ] ,
                [
        schema:name   "Miel Vander Sande" ;
        schema:email  "miel.vandersande@meemoo.be"
    ] ;
    dct:title     "Data model Events"@en ;
    dct:title     "Modèle de données Events"@fr ;
    dct:title     "Datamodel Events"@nl ;
    dct:created   "2022-06-08" ;
    dct:modified  "2022-06-08" ;
    dct:description """Data model to describe events."""@en ;
    dct:description """Modèle de données pour décrire des événements."""@fr ;
    dct:description """Datamodel voor het beschrijven van gebeurtenissen."""@nl ;
    owl:imports <http://www.loc.gov/premis/rdf/v3/> ;
    owl:imports <http://id.loc.gov/vocabulary/preservation/eventRelatedAgentRole> ;
    owl:imports <http://id.loc.gov/vocabulary/preservation/eventRelatedObjectRole> ;
    owl:imports <http://id.loc.gov/vocabulary/preservation/eventOutcome> ;
    owl:imports <http://id.loc.gov/vocabulary/preservation/eventType> ;
    pav:version "0.0.1" .

# prov classes
prov:Activity
    a owl:Class, rdfs:Class ;
    rdfs:isDefinedBy <http://www.w3.org/ns/prov-o#> ;
    rdfs:label "Activity"@en ;
    rdfs:label "Activité"@fr ;
    rdfs:label "Activiteit"@nl ;
    owl:disjointWith prov:Entity ;
    rdfs:comment "An activity is something that occurs over a period of time and acts upon or with entities; it may include consuming, processing, transforming, modifying, relocating, using, or generating entities."@en;
    rdfs:comment "Een activiteit is iets dat zich gedurende een bepaalde periode voordoet en op of met entiteiten handelt;Het kan onder meer consumeren, verwerken, transformeren, wijzigen, verplaatsen, gebruiken of genereren van entiteiten."@nl;
    rdfs:comment "Une activité est quelque chose qui se passe pendant un certain temps et qui agit sur ou avec des entités ; elle peut inclure la consommation, le traitement, la transformation, la modification, le déplacement, l'utilisation ou la génération des entités."@fr.

prov:Agent
    a owl:Class, rdfs:Class ;
    rdfs:isDefinedBy <http://www.w3.org/ns/prov-o#> ;
    rdfs:label "Agent"@en ;
    rdfs:label "Agent"@fr ;
    rdfs:label "Agent"@nl ;
    owl:disjointWith prov:InstantaneousEvent ;
    rdfs:comment "An agent is something that bears some form of responsibility for an activity taking place, for the existence of an entity, or for another agent's activity. "@en;
    rdfs:comment "Een agent is iets dat een bepaalde vorm van verantwoordelijkheid voor een activiteit neemt, voor de bestaan van een entiteit of voor de activiteit van een andere agent. "@nl;
    rdfs:comment "Un agent est quelque chose qui porte une forme de responsabilité pour une activité qui se passe, pour l'existence d'une entité ou pour l'activité d'un autre agent. "@fr.

prov:Entity
    a owl:Class, rdfs:Class ;
    rdfs:isDefinedBy <http://www.w3.org/ns/prov-o#> ;
    rdfs:label "Entity"@en ;
    rdfs:label "Entité"@fr ;
    rdfs:label "Entiteit"@nl ;
    owl:disjointWith prov:InstantaneousEvent ;
    rdfs:comment "An entity is a physical, digital, conceptual, or other kind of thing with some fixed aspects; entities may be real or imaginary. "@en;
    rdfs:comment "Een entiteit is een fysiek, digitaal, conceptueel of ander soort dingen met sommige vaste aspecten;Entiteiten kunnen echt of denkbeeldig zijn."@nl;
    rdfs:comment "Une entité est un objet physique, numérique, conceptuel ou autre de type fixe ; les entités peuvent être réelles ou imaginaires."@fr.

# prov properties
prov:generated
    a owl:ObjectProperty ;
    rdfs:domain prov:Activity ;
    rdfs:isDefinedBy <http://www.w3.org/ns/prov-o#> ;
    rdfs:label "generated"@en ;
    rdfs:label "généré"@fr ;
    rdfs:label "genereerde"@nl ;
    rdfs:range prov:Entity ;
    rdfs:subPropertyOf prov:influenced ;
    owl:inverseOf prov:wasGeneratedBy .

prov:generatedAtTime
    a owl:DatatypeProperty ;
    rdfs:domain prov:Entity ;
    rdfs:isDefinedBy <http://www.w3.org/ns/prov-o#> ;
    rdfs:label "generated at time"@en ;
    rdfs:label "généré à l'heure"@fr ;
    rdfs:label "genereerde op tijdstip"@nl ;
    rdfs:range xsd:dateTime .

prov:wasGeneratedBy
    a owl:ObjectProperty ;
    rdfs:domain prov:Entity ;
    rdfs:isDefinedBy <http://www.w3.org/ns/prov-o#> ;
    rdfs:label "was generated by"@en ;
    rdfs:label "a été généré par"@fr ;
    rdfs:label "is gegenereerd door"@nl ;
    rdfs:range prov:Activity ;
    rdfs:subPropertyOf prov:wasInfluencedBy ;
    owl:propertyChainAxiom (prov:qualifiedGeneration
        prov:activity
    ) .

prov:invalidatedAtTime
    a owl:DatatypeProperty ;
    rdfs:comment "The time at which an entity was invalidated (i.e., no longer usable)."@en ;
    rdfs:domain prov:Entity ;
    rdfs:isDefinedBy <http://www.w3.org/ns/prov-o#> ;
    rdfs:label "invalidated at time" ;
    rdfs:range xsd:dateTime .


prov:startedAtTime
    a owl:DatatypeProperty ;
    rdfs:comment "The time at which an activity started. See also prov:endedAtTime."@en ;
    rdfs:domain prov:Activity ;
    rdfs:isDefinedBy <http://www.w3.org/ns/prov-o#> ;
    rdfs:label "started at time"@en ;
    rdfs:label "démarré à l'heure"@fr ;
    rdfs:label "gestart op tijdstip"@nl ;
    rdfs:range xsd:dateTime .

prov:wasAssociatedWith
    a owl:ObjectProperty ;
    rdfs:comment "An prov:Agent that had some (unspecified) responsibility for the occurrence of this prov:Activity."@en ;
    rdfs:domain prov:Activity ;
    rdfs:isDefinedBy <http://www.w3.org/ns/prov-o#> ;
    rdfs:label "was associated with"@en ;
    rdfs:label "a été associé à"@fr ;
    rdfs:label "is geassocieerd met"@nl ;
    rdfs:range prov:Agent ;
    rdfs:subPropertyOf prov:wasInfluencedBy ;
    owl:propertyChainAxiom (prov:qualifiedAssociation
        prov:agent
    ) .

prov:wasAttributedTo
    a owl:ObjectProperty ;
    rdfs:comment "Attribution is the ascribing of an entity to an agent."@en ;
    rdfs:domain prov:Entity ;
    rdfs:isDefinedBy <http://www.w3.org/ns/prov-o#> ;
    rdfs:label "was attributed to"@en ;
    rdfs:label "a été attribué à"@fr ;
    rdfs:label "is toegekend aan"@nl ;
    rdfs:range prov:Agent ;
    rdfs:subPropertyOf prov:wasInfluencedBy ;
    owl:propertyChainAxiom (prov:qualifiedAttribution
        prov:agent
    ) .

prov:used
    a owl:ObjectProperty ;
    rdfs:comment "A prov:Entity that was used by this prov:Activity. For example, :baking prov:used :spoon, :egg, :oven ."@en ;
    rdfs:domain prov:Activity ;
    rdfs:isDefinedBy <http://www.w3.org/ns/prov-o#> ;
    rdfs:label "used"@en ;
    rdfs:label "a utilisé"@fr ;
    rdfs:label "gebruikte"@nl ;
    rdfs:range prov:Entity ;
    rdfs:subPropertyOf prov:wasInfluencedBy ;
    owl:propertyChainAxiom (prov:qualifiedUsage
        prov:entity
    ) .

# premis classes

# vraag: zijn dit bij ons personen en organisaties uit het organisatiemodel?
# zo ja, dan dekt de naam 'organisatiemodel' de lading misschien niet zo goed?
premis:Agent  a owl:Class, rdfs:Class ;
  rdfs:label "Agent"@en ;
  rdfs:label "Acteur"@fr ;
  rdfs:label "Agent"@nl ;
  rdfs:comment """Actor (human, machine, or software) associated with one or more Event and/or Rights statement associated with a digital object."""@en ;
  rdfs:comment """Acteur (humain, machine ou logiciel) associé à un ou plusieurs Events et/ou déclarations de Rights associés à un objet numérique/digital."""@fr ;
  rdfs:comment """Agens (mens, machine of software) geassocieerd met één of meer Events en/of Rights uitdrukkingen geassocieerd met een digitaal object."""@nl ;
  rdfs:subClassOf prov:Agent, foaf:Agent ;
  rdfs:isDefinedBy <http://www.loc.gov/premis/rdf/v3/> .

premis:SoftwareAgent
  a owl:Class, rdfs:Class ;
  rdfs:label "Software agent"@en ;
  rdfs:label "Logiciel acteur"@fr ;
  rdfs:label "Software agent"@nl ;
  rdfs:comment """Software agent (e.g., a computer program) that is associated with one or more Event and/or Rights statement associated with a digital object."""@en ;
  rdfs:comment """Logiciel acteur (e.g., un programme informatique) associé à un ou plusieurs Events et/ou déclarations de Rights associés à un objet numérique/digital."""@fr ;
  rdfs:comment """Softwareagent (bijv. Een computerprogramma) dat is gekoppeld aan een of meer evenement- en/of rechtenverklaring die aan een digitaal object is gekoppeld."""@nl ;
  rdfs:subClassOf premis:Agent, prov:SoftwareAgent ;
  owl:disjointWith premis:HardwareAgent, premis:Organization, premis:Person ;
  rdfs:isDefinedBy <http://www.loc.gov/premis/rdf/v3/> .

premis:HardwareAgent
  a owl:Class, rdfs:Class ;
  rdfs:label "Hardware agent"@en ;
  rdfs:label "Matériel acteur"@fr ;
  rdfs:label "Hardware agent"@nl ;
  rdfs:comment """Hardware agent (e.g., a computer) that is associated with one or more Event and/or Rights statement associated with a digital object."""@en ;
  rdfs:comment """Matériel acteur (e.g., un ordinateur) associé à un ou plusieurs Events et/ou déclarations de Rights associés à un objet numérique/digital."""@fr ;
  rdfs:comment """Hardwareagent (bijv. Een computer) dat is gekoppeld aan een of meer evenement- en/of rechtenverklaring die aan een digitaal object is gekoppeld."""@nl ;
  rdfs:subClassOf premis:Agent ;
  owl:sameAs <http://id.loc.gov/vocabulary/preservation/agentType/har> ;
  owl:disjointWith premis:Organization, premis:Person, premis:SoftwareAgent ;
  rdfs:isDefinedBy <http://www.loc.gov/premis/rdf/v3/> .

premis:Event  a owl:Class, rdfs:Class ;
  rdfs:label "Event"@en ;
  rdfs:label "Événement"@fr ;
  rdfs:label "Gebeurtenis"@nl ;
  rdfs:comment "Action performed within or outside the repository that affects its capability to preserve Objects over the long term."@en ;
  rdfs:comment "Action réalisée à l'intérieur ou à l'extérieur du dépôt qui affecte sa capacité à préserver des objets sur le long terme."@fr ;
  rdfs:comment "Handeling uitgevoerd binnen of buiten het archief die het vermogen beïnvloedt om objecten op lange termijn te bewaren."@nl ;
  rdfs:subClassOf prov:Activity ;
  rdfs:isDefinedBy <http://www.loc.gov/premis/rdf/v3/> ;
  rdfs:seeAlso <http://id.loc.gov/vocabulary/preservation/eventType> .

premis:OutcomeStatus  a owl:Class, rdfs:Class ;
  rdfs:label "Outcome status"@en ;
  rdfs:label "Statut de résultat"@fr ;
  rdfs:label "Uitkomststatus"@nl ;
  rdfs:comment "Overall result of the Event in terms of success, partial success, or failure."@en ;
  rdfs:comment "Résultat global de l'événement en termes de succès, de succès partiel ou d'échec."@fr ;
  rdfs:comment "Algemeen resultaat van het Event in termen van succes, gedeeltelijk succes of falen."@nl ;
  rdfs:isDefinedBy <http://www.loc.gov/premis/rdf/v3/> ;
  rdfs:seeAlso <http://id.loc.gov/vocabulary/preservation/eventOutcome> .

# premis properties

premis:endDate  a owl:DatatypeProperty ;
  rdfs:label "end date"@en ;
  rdfs:label "date de fin"@en ;
  rdfs:label "einddatum"@en ;
  rdfs:domain [
    a owl:Class, rdfs:Class ;
    owl:unionOf (
     premis:RightsStatus
     premis:Rule
   )
  ] ;
  rdfs:subPropertyOf dct:date ;
  rdfs:isDefinedBy <http://www.loc.gov/premis/rdf/v3/> .

premis:note  a owl:DatatypeProperty ;
  rdfs:label "has note"@en ;
  rdfs:label "a note"@en ;
  rdfs:label "heeft nota"@en ;
  rdfs:range rdfs:Literal ;
  rdfs:subPropertyOf dct:description ;
  rdfs:isDefinedBy <http://www.loc.gov/premis/rdf/v3/> .

premis:outcome  a owl:ObjectProperty ;
  rdfs:label "has outcome"@en ;
  rdfs:label "a résultat"@fr ;
  rdfs:label "heeft resultaat"@nl ;
  rdfs:domain premis:Event ;
  rdfs:range premis:OutcomeStatus ;
  rdfs:isDefinedBy <http://www.loc.gov/premis/rdf/v3/> .

premis:outcomeNote  a owl:DatatypeProperty ;
  rdfs:label "has outcome note"@en ;
  rdfs:label "a note de résultat"@fr ;
  rdfs:label "heeft resultaatnota"@nl ;
  rdfs:domain premis:Event ;
  rdfs:range rdfs:Literal ;
  rdfs:subPropertyOf premis:note ;
  rdfs:isDefinedBy <http://www.loc.gov/premis/rdf/v3/> .

premis:startDate    a owl:DatatypeProperty ;
  rdfs:label "start date"@en ;
  rdfs:label "date de début"@fr ;
  rdfs:label "startdatum"@nl ;
  rdfs:domain [
    a owl:Class, rdfs:Class ;
    owl:unionOf (
     premis:RightsStatus
     premis:Rule
   )
  ] ;
  rdfs:subPropertyOf dct:date ;
  rdfs:isDefinedBy <http://www.loc.gov/premis/rdf/v3/> .

# premis events classes

# premis events properties

evtObjRole:sou a owl:ObjectProperty ;
    rdfs:domain premis:Event ;
    rdfs:range premis:Object ;
    rdfs:label "source"@en;
    rdfs:label "source"@fr;
    rdfs:label "bron"@nl;
    rdfs:subPropertyOf prov:used ;
    rdfs:comment "The object in relation to the described event that existed prior to that event and was used by it."@en;
    rdfs:comment "L'objet dans la relation à l'événement décrit et qui existait avant cet événement et qui l'utilisait."@fr;
    rdfs:comment "Het object in de relatie met het geschreven event dat bestond voor dat event en die het gebruikt."@nl.

evtObjRole:out a owl:ObjectProperty ;
    rdfs:domain premis:Event ;
    rdfs:range premis:Object ;
    rdfs:subPropertyOf prov:generated ;
    rdfs:comment "The object in relation to the described event is the outcome of that event."@en ;
    rdfs:comment "L'objet dans la relation à l'événement décrit est le résultat de cet événement."@fr ;
    rdfs:comment "Het object in de relatie met het geschreven event is het resultaat van dat event."@nl;
    rdfs:label "outcome"@en ;
    rdfs:label "résultat"@fr ;
    rdfs:label "uitkomst"@nl.

# meemoo classes



# meemoo properties